spec-compilers/fstar/poly1305.fst
@@ -8,27 +8,11 @@ let blocksize = 0x10
 let block_t = bytes_t 0x10 
 let key_t = bytes_t 0x20 
 let tag_t = bytes_t 0x10 
-let subblock = refine3 vlbytes Lambda(args=arguments(args=arg(arg='x',
-               annotation=None,
-               type_comment=None),
-               vararg=None,
-               kwonlyargs=,
-               kw_defaults=,
-               kwarg=None,
-               defaults=),
-               body=((length x) <= 0x10)) 
-let subblock_t = subblock 
+type subblock_t = x:vlbytes_t{(length x <= 0x10)}
+
 let p130m5 = ((0x2 **. 0x82) -. 0x5) 
-let felem = refine3 nat Lambda(args=arguments(args=arg(arg='x',
-            annotation=None,
-            type_comment=None),
-            vararg=None,
-            kwonlyargs=,
-            kw_defaults=,
-            kwarg=None,
-            defaults=),
-            body=(x < p130m5)) 
-let felem_t = felem 
+type felem_t = x:nat{(x < p130m5)}
+
 let felem (x:nat) : felem_t =
   (x %. p130m5) 
 let fadd (x:felem_t) (y:felem_t) : felem_t =
